Add lemmas to specify valid_ocmp in decls

src/arch/x64/X64.Vale.Lemmas_i.fst
@@ -54,6 +54,13 @@ let lemma_cmp_ge s o1 o2 = ()
 let lemma_cmp_lt s o1 o2 = ()
 let lemma_cmp_gt s o1 o2 = ()
 
+let lemma_valid_cmp_eq s o1 o2 = ()
+let lemma_valid_cmp_ne s o1 o2 = ()
+let lemma_valid_cmp_le s o1 o2 = ()
+let lemma_valid_cmp_ge s o1 o2 = ()
+let lemma_valid_cmp_lt s o1 o2 = ()
+let lemma_valid_cmp_gt s o1 o2 = ()
+
 let lemma_merge_total (b0:codes) (s0:state) (f0:fuel) (sM:state) (fM:fuel) (sN:state) =
   let f = if f0 > fM then f0 else fM in
   increase_fuel (Cons?.hd b0) s0 f0 sM f;
